prove lift_ok in RefinementAlloc.v
required tweaking txn_valid to be more reasonable

src/Examples/Logging2/Liftable.v
@@ -19,6 +19,26 @@ Section liftable.
 
   Definition heapT := @gen_heapG L V Σ _ _.
 
+  Definition Conflicting (P0 P1 : L -> V -> iProp Σ) :=
+    forall a0 v0 a1 v1,
+      ( P0 a0 v0 -∗ P1 a1 v1 -∗ ⌜ a0 ≠ a1 ⌝ )%I.
+
+  Lemma big_sepM_disjoint_pred (m0 m1 : gmap L V) P0 P1 :
+    Conflicting P0 P1 ->
+    ( ( [∗ map] a↦v ∈ m0, P0 a v ) -∗
+      ( [∗ map] a↦v ∈ m1, P1 a v ) -∗
+      ⌜ m0 ##ₘ m1 ⌝ )%I.
+  Proof.
+    iIntros (Hc) "H0 H1".
+    iIntros (i).
+    unfold option_relation.
+    destruct (m0 !! i) eqn:H0; destruct (m1 !! i) eqn:H1; try solve [ iPureIntro; auto ].
+    iDestruct (big_sepM_lookup with "H0") as "H0"; eauto.
+    iDestruct (big_sepM_lookup with "H1") as "H1"; eauto.
+    iDestruct (Hc with "H0 H1") as %Hcc.
+    congruence.
+  Qed.
+
   Lemma mapsto_disjoint h (a0 a1 : L) (v0 v1 : V) :
     ( mapsto (Σ := Σ) (hG := h) a0 1 v0 -∗
       mapsto (Σ := Σ) (hG := h) a1 1 v1 -∗
@@ -37,14 +57,11 @@ Section liftable.
       ( [∗ map] a↦v ∈ m1, mapsto (Σ := Σ) (hG := h) a 1 v ) -∗
       ⌜ m0 ##ₘ m1 ⌝ )%I.
   Proof.
+    apply big_sepM_disjoint_pred.
+    unfold Conflicting; intros.
     iIntros "H0 H1".
-    iIntros (i).
-    unfold option_relation.
-    destruct (m0 !! i) eqn:H0; destruct (m1 !! i) eqn:H1; try solve [ iPureIntro; auto ].
-    iDestruct (big_sepM_lookup with "H0") as "H0"; eauto.
-    iDestruct (big_sepM_lookup with "H1") as "H1"; eauto.
     iDestruct (mapsto_disjoint with "H0 H1") as %Hc.
-    congruence.
+    iPureIntro; auto.
   Qed.
 
   Class Liftable (P : heapT -> iProp Σ) := liftable :
